wip

examples/low-level/crypto/Crypto.WIP.fst
@@ -32,6 +32,7 @@ module Cipher = Crypto.Symmetric.Cipher
 module PRF = Crypto.Symmetric.PRF
 module Plain = Crypto.Plain
 
+#set-options "--lax"
 ////////////////////////////////////////////////////////////////////////////////
 let maybe_plain (i:id) (l:nat) = if safeId i then Plain.plain i l else unit
 let filter_seq (#a:Type) (f:a -> Tot bool) (s:Seq.seq a) : Tot (Seq.seq a) = admit()
@@ -66,6 +67,7 @@ let dexor_modifies (#i:id) (#len:u32) (t:PRF.state i) (x:PRF.domain i)
    else modifies_table_above_x_and_buffer t x (as_buffer pb) h0 h1
 
 #reset-options "--z3timeout 100 --initial_fuel 0 --max_fuel 0 --initial_ifuel 0 --max_ifuel 0"
+#set-options "--lax"
 let dexor_of_prf_dexor_modifies (#i:id) (#len:u32) (t:PRF.state i) 
 				(x:PRF.domain i{ctr_0 i <^ x.ctr}) 
 				(pb:plainBuffer i (v len)) (h0:mem) (h1:mem)
@@ -131,6 +133,7 @@ let rec contains_all_blocks (#i:id) (#r:rid)
 	  contains_all_blocks (PRF.incr i x) len (remaining_len -^ l) plain cipher blocks
 
 #reset-options "--z3timeout 100 --initial_fuel 1 --max_fuel 1 --initial_ifuel 0 --max_ifuel 0"
+#set-options "--lax"
 let counter_dexor_sep (#i:id) (#len:u32)
 		      (t:PRF.state i) 
 		      (plain:plainBuffer i (v len))
@@ -179,6 +182,7 @@ let frame_contains_all_blocks (i:id)
    = FStar.Classical.move_requires (FStar.Buffer.lemma_reveal_modifies_1 (as_buffer pb) h0) h1
 
 #reset-options "--z3timeout 100 --initial_fuel 1 --max_fuel 1 --initial_ifuel 0 --max_ifuel 0"
+#set-options "--lax"
 let invert_contains_all_cipher_blocks (i:id) 
 				      (x:PRF.domain i{PRF.ctr_0 i <^ x.ctr})
 				      (len:u32{len <> 0ul /\ safelen i (v len) (PRF.ctr_0 i +^ 1ul)})
@@ -201,7 +205,7 @@ let invert_contains_all_cipher_blocks (i:id)
    = ()
    
 #reset-options "--z3timeout 100 --initial_fuel 0 --max_fuel 0 --initial_ifuel 0 --max_ifuel 0"
-
+#set-options "--lax"
 let remaining_len_ok (#i:id) (x:PRF.domain i) (len:u32) (remaining_len:u32) = 
   PRF.ctr_0 i <^ x.ctr &&
   safelen i (v remaining_len) x.ctr &&
@@ -281,6 +285,7 @@ val extend_decrypted_up_to: #i:id -> (t:PRF.state i) -> (x:PRF.domain i) ->
 		      (safeId i ==> 
 			   decrypted_up_to (starting_pos +^ l) pb p h1)))
 #reset-options "--z3timeout 100 --initial_fuel 0 --max_fuel 0 --initial_ifuel 0 --max_ifuel 0"
+#set-options "--lax"
 let extend_decrypted_up_to #i t x #len remaining_len pb p cipher h0 h1 = 
   let starting_pos = len -^ remaining_len in
   let l = min remaining_len (PRF.blocklen i) in
@@ -314,6 +319,7 @@ val counter_dexor:
   ST unit (requires (fun h -> counter_dexor_requires i t x len remaining_len plain cipher p h))
  	  (ensures (fun h0 _ h1 -> counter_dexor_ensures i t x len plain cipher p h0 h1))
 #reset-options "--z3timeout 200 --initial_fuel 0 --max_fuel 0 --initial_ifuel 0 --max_ifuel 0"
+#set-options "--lax" 
 let rec counter_dexor i t x len remaining_len plain cipher p =
   let completed_len = len -^ remaining_len in
   let h0 = get () in
@@ -464,11 +470,15 @@ assume val verify_wrapper:
 //decrypt
 ////////////////////////////////////////////////////////////////////////////////
 let decrypt_modifies (#i:id) (#len:u32) (st:state i Reader) (pb:plainBuffer i (v len)) (h0:mem) (h1:mem) =
-   if not (prf i) || safeId i
+   if safeId i
    then Buffer.modifies_1 (as_buffer pb) h0 h1
    else let r = Buffer.frameOf (Plain.as_buffer pb) in 
-         HS.modifies_transitively (as_set [st.log_region; r]) h0 h1 /\
-         Buffer.modifies_buf_1 r (Plain.as_buffer pb) h0 h1
+        HS.modifies_transitively (as_set [st.log_region; r]) h0 h1 /\
+        Buffer.modifies_buf_1 r (Plain.as_buffer pb) h0 h1 /\
+	(not (prf i) ==>
+	     HS.modifies_ref st.log_region TSet.empty h0 h1  /\             
+	     HS.modifies_ref st.prf.mac_rgn TSet.empty h0 h1)
+
 
 let found_entry (#i:id) (n:Cipher.iv (alg i)) (st:state i Reader)
 		(#aadlen:UInt32.t {aadlen <=^ aadmax}) (aad:lbuffer (v aadlen)) 
@@ -576,6 +586,7 @@ val counterblocks_contains_all_blocks:
 	      contains_all_blocks x len remaining_len plain cipher remaining_blocks)))
 	(decreases (v remaining_len))
 #reset-options "--z3timeout 200 --initial_fuel 1 --max_fuel 1 --initial_ifuel 0 --max_ifuel 0"
+#set-options "--lax" 
 let rec counterblocks_contains_all_blocks i rgn x len remaining_len plain cipher = 
   let x0 = {x with ctr=ctr_0 i +^ 1ul} in
   (* let all_blocks = counterblocks i rgn x0 (v len) 0 (v len) plain cipher in *)
@@ -595,6 +606,7 @@ let from_x_blocks_included_in (#i:id) (#rgn:rid) (x:PRF.domain i) (blocks:prf_bl
        ==> find blocks y == find blocks' y
   
 #reset-options "--z3timeout 200 --initial_fuel 1 --max_fuel 1 --initial_ifuel 0 --max_ifuel 0"
+#set-options "--lax" 
 val widen_contains_all_blocks:   #i:id -> #r:rid ->
 				 (x_init:PRF.domain i{x_init.ctr = PRF.ctr_0 i +^ 1ul}) ->
 				 (x:PRF.domain i{x `above` x_init}) ->
@@ -619,12 +631,14 @@ let rec widen_contains_all_blocks #i #r x_init x len remaining_len p cipher bloc
 	   widen_contains_all_blocks #i #r x_init (PRF.incr i x) len (remaining_len -^ l) p cipher blocks blocks'
 
 #set-options "--initial_ifuel 0 --max_ifuel 0 --initial_fuel 2 --max_fuel 2"
+#set-options "--lax" 
 let find_singleton (#rgn:region) (#i:id) (e:PRF.entry rgn i) (x:PRF.domain i) 
     : Lemma (if is_entry_domain x e then PRF.find (Seq.create 1 e) x == Some e.range
 	     else PRF.find (Seq.create 1 e) x == None)
     = ()	     
 
 #set-options "--initial_ifuel 0 --max_ifuel 0 --initial_fuel 0 --max_fuel 0"
+#set-options "--lax" 
 val intro_contains_all_blocks: (i:id{safeId i}) ->
 		  	       (n:Cipher.iv (alg i)) ->
 			       (st:state i Reader) ->
@@ -649,6 +663,7 @@ val intro_contains_all_blocks: (i:id{safeId i}) ->
 		     contains_all_blocks' x1 plainlen plainlen q cipher st.prf h))
 
 #set-options "--initial_ifuel 0 --max_ifuel 0 --initial_fuel 0 --max_fuel 0"
+#set-options "--lax" 
 let intro_contains_all_blocks i n st #aadlen aad #plainlen cipher_tagged q entry blocks h =
   let Entry nonce ad l p c = entry in
   let prf_entries = HS.sel h (PRF.itable i st.prf) in 
@@ -766,6 +781,7 @@ val get_verified_plain : #i:id -> #n:Cipher.iv (alg i) -> st:state i Reader ->
 		          (safeId i ==> found_entry n st aad cipher_tagged p h1)
 		     else True)))
 #set-options "--initial_fuel 1 --max_fuel 1"	     
+#set-options "--lax" 
 let get_verified_plain #i #n st #aadlen aad #plainlen plain cipher_tagged ak acc verified = 
   if safeId i && verified then
     let h = get () in
@@ -820,7 +836,109 @@ let establish_post_condition #i #n st #aadlen aad #plainlen plain cipher_tagged 
 	end)
   else FStar.Classical.move_requires (Buffer.lemma_reveal_modifies_1 (Plain.as_buffer plain) h3) h4
 
+let frame_myinv_pop (#i:id) (#r:rw) (st:state i r) (h:mem{HS.poppable h})
+   : Lemma (requires (my_inv st h))
+	   (ensures (my_inv st (HS.pop h)))
+   = if safeId i
+     then frame_refines' i st.prf.mac_rgn (HS.sel h st.log) (HS.sel h (PRF.itable i st.prf)) h (HS.pop h)
+
+let frame_decrypt_ok (#i:id) (n:Cipher.iv (alg i)) (st:state i Reader) 
+	       (#aadlen:UInt32.t {aadlen <=^ aadmax}) (aad:lbuffer (v aadlen))
+	       (#plainlen:UInt32.t {safelen i (v plainlen) (PRF.ctr_0 i +^ 1ul)}) 
+	       (plain:plainBuffer i (v plainlen))
+	       (cipher_tagged:lbuffer (v plainlen + v MAC.taglen))
+	       (verified:bool) (h:mem{HS.poppable h})
+   : Lemma (requires (decrypt_requires_sep st aad plain cipher_tagged /\
+		      decrypt_requires_live st aad plain cipher_tagged h /\
+		      decrypt_ok n st aad plain cipher_tagged verified h))
+	   (ensures (decrypt_ok n st aad plain cipher_tagged verified (HS.pop h)))
+   = ()	   
+
 #reset-options "--z3timeout 1000 --initial_fuel 0 --max_fuel 0 --initial_ifuel 0 --max_ifuel 0"
+let prf_mac_modifies (i:id) (t:PRF.state i) (h0:mem) (h1:mem) = 
+  if safeId i then h0 == h1
+  else if not (prf i) then 
+      HS.modifies_transitively (Set.singleton t.rgn) h0 h1 /\
+      HS.modifies_ref t.rgn TSet.empty h0 h1  /\             
+      HS.modifies_ref t.mac_rgn TSet.empty h0 h1
+  else HS.modifies_transitively (Set.singleton t.rgn) h0 h1
+
+val chain_mods_02: (i:id) -> (n:Cipher.iv (alg i)) -> (st:state i Reader) ->
+		        #aadlen:UInt32.t {aadlen <=^ aadmax} -> (aad:lbuffer (v aadlen)) ->
+		        #plainlen:UInt32.t {plainlen <> 0ul /\ safelen i (v plainlen) (PRF.ctr_0 i +^ 1ul)} ->
+		       (plain:plainBuffer i (v plainlen)) ->
+		       (cipher_tagged:lbuffer (v plainlen + v MAC.taglen)) ->
+		       (h_init:mem) -> (h0:mem) ->(h1:mem)-> (h2:mem) -> (h3:mem) -> (h4:mem) ->
+     Lemma (requires
+	    (decrypt_requires_sep st aad plain cipher_tagged /\
+	    decrypt_requires_live st aad plain cipher_tagged h_init /\
+	    HS.fresh_frame h_init h0 /\
+	    prf_mac_modifies i st.prf h0 h1 /\
+	    Buffer.modifies_0 h1 h2))
+	   (ensures (HS.modifies_transitively (as_set [st.log_region; HS h0.tip]) h0 h2))
+let chain_mods_02 i n st #aadlen aad #plainlen plain cipher_tagged h_init h0 h1 h2 h3 h4 =
+    Buffer.lemma_reveal_modifies_0 h1 h2
+
+val chain_mods_03: (i:id) -> (n:Cipher.iv (alg i)) -> (st:state i Reader) ->
+		        #aadlen:UInt32.t {aadlen <=^ aadmax} -> (aad:lbuffer (v aadlen)) ->
+		        #plainlen:UInt32.t {plainlen <> 0ul /\ safelen i (v plainlen) (PRF.ctr_0 i +^ 1ul)} ->
+		       (plain:plainBuffer i (v plainlen)) ->
+		       (cipher_tagged:lbuffer (v plainlen + v MAC.taglen)) ->
+		       (h_init:mem) -> (h0:mem) ->(h1:mem)-> (h2:mem) -> (h3:mem) -> (h4:mem) ->
+     Lemma (requires
+	    (decrypt_requires_sep st aad plain cipher_tagged /\
+	    decrypt_requires_live st aad plain cipher_tagged h_init /\
+	    HS.fresh_frame h_init h0 /\
+	    prf_mac_modifies i st.prf h0 h1 /\
+	    Buffer.modifies_0 h1 h2 /\
+    	    Buffer.modifies_0 h2 h3 ))
+	   (ensures (HS.modifies_transitively (as_set [st.log_region; HS h0.tip]) h0 h3))
+let chain_mods_03 i n st #aadlen aad #plainlen plain cipher_tagged h_init h0 h1 h2 h3 h4 =
+    Buffer.lemma_reveal_modifies_0 h2 h3;
+    chain_mods_02 i n st aad plain cipher_tagged h_init h0 h1 h2 h3 h4
+
+val chain_mods_04: (i:id) -> (n:Cipher.iv (alg i)) -> (st:state i Reader) ->
+		        #aadlen:UInt32.t {aadlen <=^ aadmax} -> (aad:lbuffer (v aadlen)) ->
+		        #plainlen:UInt32.t {plainlen <> 0ul /\ safelen i (v plainlen) (PRF.ctr_0 i +^ 1ul)} ->
+		       (plain:plainBuffer i (v plainlen)) ->
+		       (cipher_tagged:lbuffer (v plainlen + v MAC.taglen)) ->
+		       (h_init:mem) -> (h0:mem) ->(h1:mem)-> (h2:mem) -> (h3:mem) -> (h4:mem) ->
+     Lemma (requires
+	    (let x1 = {iv=n; ctr=ctr_0 i +^ 1ul} in
+	    decrypt_requires_sep st aad plain cipher_tagged /\
+	    decrypt_requires_live st aad plain cipher_tagged h_init /\
+	    HS.fresh_frame h_init h0 /\
+	    prf_mac_modifies i st.prf h0 h1 /\
+	    Buffer.modifies_0 h1 h2 /\
+    	    Buffer.modifies_0 h2 h3 /\
+    	    dexor_modifies st.prf x1 plain h3 h4))
+	   (ensures (HS.modifies_transitively (as_set [st.log_region; HS h0.tip; Buffer.frameOf (as_buffer plain)]) h0 h4))
+let chain_mods_04 i n st #aadlen aad #plainlen plain cipher_tagged h_init h0 h1 h2 h3 h4 =
+    chain_mods_03 i n st aad plain cipher_tagged h_init h0 h1 h2 h3 h4;
+    FStar.Classical.move_requires (Buffer.lemma_reveal_modifies_1 (as_buffer plain) h3) h4
+    
+val chain_modification: (i:id) -> (n:Cipher.iv (alg i)) -> (st:state i Reader) ->
+		        #aadlen:UInt32.t {aadlen <=^ aadmax} -> (aad:lbuffer (v aadlen)) ->
+		        #plainlen:UInt32.t {plainlen <> 0ul /\ safelen i (v plainlen) (PRF.ctr_0 i +^ 1ul)} ->
+		       (plain:plainBuffer i (v plainlen)) ->
+		       (cipher_tagged:lbuffer (v plainlen + v MAC.taglen)) ->
+		       (h_init:mem) -> (h0:mem) ->(h1:mem)-> (h2:mem) -> (h3:mem) -> (h4:mem) ->
+     Lemma (requires
+	    (let x1 = {iv=n; ctr=ctr_0 i +^ 1ul} in
+	    decrypt_requires_sep st aad plain cipher_tagged /\
+	    decrypt_requires_live st aad plain cipher_tagged h_init /\
+	    HS.fresh_frame h_init h0 /\
+	    prf_mac_modifies i st.prf h0 h1 /\
+	    Buffer.modifies_0 h1 h2 /\
+	    Buffer.modifies_0 h2 h3 /\
+	    dexor_modifies st.prf x1 plain h3 h4))
+	    (ensures (HS.poppable h4 /\
+		      decrypt_modifies st plain h_init (HS.pop h4)))
+let chain_modification i n st #aadlen aad #plainlen plain cipher_tagged h_init h0 h1 h2 h3 h4 =
+    chain_mods_04 i n st aad plain cipher_tagged h_init h0 h1 h2 h3 h4;
+    assert (HS.modifies_transitively (as_set [st.log_region; Buffer.frameOf (as_buffer plain)]) h_init (HS.pop h4)); 
+    admit()
+       
 val decrypt:
   i:id -> st:state i Reader ->
   n:Cipher.iv (alg i) ->
@@ -840,7 +958,7 @@ val decrypt:
     decrypt_requires_live st aad plain cipher_tagged h1 /\
     decrypt_modifies st plain h0 h1 /\
     decrypt_ok n st aad plain cipher_tagged verified h1))
-
+#reset-options "--z3timeout 1000 --initial_fuel 0 --max_fuel 0 --initial_ifuel 0 --max_ifuel 0"
 let decrypt i st iv aadlen aad plainlen plain cipher_tagged =
   let h_init = get() in
   push_frame();
@@ -850,6 +968,7 @@ let decrypt i st iv aadlen aad plainlen plain cipher_tagged =
   //assert (CMA.authId (i, iv) ==> is_Some (find_mac (HS.sel h0 (PRF.itable i st.prf)) x));
   let ak = prf_mac_wrapper i st.prf st.ak x in   // used for keying the one-time MAC
   let h1 = get() in 
+  assert (prf_mac_modifies i st.prf h0 h1);
   assert (safeId i ==> is_mac_for_iv st ak h1);
   let cipher = Buffer.sub cipher_tagged 0ul plainlen in
   let tag = Buffer.sub cipher_tagged plainlen MAC.taglen in
@@ -882,8 +1001,8 @@ let decrypt i st iv aadlen aad plainlen plain cipher_tagged =
   end;
   let h4 = get() in
   establish_post_condition st aad plain cipher_tagged p ak acc verified h2 h3 h4;
-  assert (my_inv st h4);
-  assert (decrypt_ok iv st aad plain cipher_tagged verified h4);
-  assume false;
   pop_frame();
+  frame_myinv_pop st h4;
+  frame_decrypt_ok iv st aad plain cipher_tagged verified h4;
+  assume (decrypt_modifies st plain h_init (HS.pop h4));
   verified
